kalloc/Verif_kalloc_kfree.v
@@ -18,14 +18,15 @@ destruct (eq_dec new_head nullval).
 - forward_if.
     * Intros. forward. unfold type_kalloc_token. Intros. rewrite kalloc_token_sz_split. Intros. 
      rewrite memory_block_data_at_; auto. forward. forward. 
-     entailer. rewrite mem_mgr_split. refold_freelistrep. entailer!.
-     right; split; auto. unfold not; auto_contradict.
+     entailer. rewrite mem_mgr_split. refold_freelistrep_safe. entailer!. split.
+     right; split; auto. unfold not; auto_contradict. constructor; auto.
+     destruct H as [HH1 [HH2 | HH2]]; auto.
     * forward. entailer.
 Qed.
 
 Lemma body_kalloc: semax_body KAFVprog KAFGprog f_kalloc (kalloc_spec (KAF_APD) t_run).
 Proof. start_function.
-rewrite mem_mgr_split. Intros. forward.
+rewrite mem_mgr_split. unfold freelistrep_safe. Intros. forward. 
 forward_if (
     PROP  ( )
     LOCAL (
@@ -46,24 +47,26 @@ forward_if (
     )
 )%assert.
 - destruct H3 as [[H0011 H0012] | [H0021 H0022]].
-    + rewrite H0012 in H4; auto_contradict.
+    + rewrite H0012 in H5; auto_contradict.
     + destruct ls; auto_contradict.
-    refold_freelistrep. Intros.
+    refold_freelistrep_safe. Intros.
     forward. forward.
     entailer.
     rewrite mem_mgr_split. Intros. 
-    refold_freelistrep. if_tac.
-    * rewrite H11 in H0022; auto_contradict.
+    refold_freelistrep_safe. if_tac.
+    * rewrite H12 in H0022; auto_contradict.
     * entailer. Exists v ls. entailer. unfold type_kalloc_token.
     rewrite kalloc_token_sz_split. rewrite mem_mgr_split. entailer!.
     -- destruct ls.
-        ++ left; split; auto. rewrite <- H9; auto.
+        ++ left; split; auto. rewrite <- H10; auto.
         ++ right. split.
             **  unfold not. intros; auto_contradict.
-            ** rewrite <- H10. unfold not; intros; auto_contradict.
-    -- apply data_at_memory_block.
+            ** rewrite <- H11. unfold not; intros; auto_contradict.
+    -- unfold freelistrep_safe. entailer!. rewrite NoDup_cons_iff in H4. destruct H4. auto. apply data_at_memory_block.
 -forward. destruct (eq_dec original_freelist_pointer nullval) eqn:e1; auto_contradict. entailer.
-rewrite mem_mgr_split. entailer.
-- if_tac; forward.
+rewrite mem_mgr_split. unfold freelistrep_safe. entailer.
+- if_tac; forward. destruct H3 as [[HH1 HH2] | [HH1 HH2]]; auto_contradict.
+    Exists next ls'. entailer!.
+    rewrite NoDup_cons_iff in H4. destruct H4. unfold not in H4. apply H4. simpl. right; auto.
 Qed.
 
